theories/Hoareproof0.v
@@ -101,18 +101,18 @@ Section CANCEL.
     ss. rewrite IHmds0. auto.
   Qed.
 
-  Lemma initial_p_eq:
-    ModSemL.initial_p_state ms_tgt = ModSemL.initial_p_state ms_mid.
-  Proof.
-    unfold ModSemL.initial_p_state. extensionality mn.
-    pose proof sk_eq.
-    unfold ms_tgt, ms_mid, mds_tgt, mds_mid, ModL.enclose.
-    unfold mds_mid, mds_tgt in H. rewrite H.
-    generalize (ModL.sk (Mod.add_list (List.map (SMod.to_mid (stb sk)) mds))). i.
-    rewrite ! Mod.add_list_initial_mrs.
-    generalize mds. clear. i. induction mds0; auto.
-    ss. rewrite eq_rel_dec_correct in *. des_ifs.
-  Qed.
+  (* Lemma initial_p_eq: *)
+  (*   ModSemL.initial_p_state ms_tgt = ModSemL.initial_p_state ms_mid. *)
+  (* Proof. *)
+  (*   unfold ModSemL.initial_p_state. extensionality mn. *)
+  (*   pose proof sk_eq. *)
+  (*   unfold ms_tgt, ms_mid, mds_tgt, mds_mid, ModL.enclose. *)
+  (*   unfold mds_mid, mds_tgt in H. rewrite H. *)
+  (*   generalize (ModL.sk (Mod.add_list (List.map (SMod.to_mid (stb sk)) mds))). i. *)
+  (*   rewrite ! Mod.add_list_initial_mrs. *)
+  (*   generalize mds. clear. i. induction mds0; auto. *)
+  (*   ss. rewrite eq_rel_dec_correct in *. des_ifs. *)
+  (* Qed. *)
 
   Lemma fns_eq:
     (List.map fst (ModSemL.fnsems (ModL.enclose (Mod.add_list mds_tgt))))
@@ -183,14 +183,18 @@ Section CANCEL.
     { right. esplits; et. }
   Qed.
 
-  Let W: Type := (r_state * p_state).
-  Let rsum: r_state -> Σ :=
-    fun '(mrs_tgt, frs_tgt) => (fold_left (⋅) (List.map (mrs_tgt <*> fst) ms_tgt.(ModSemL.initial_mrs)) ε) ⋅ (fold_left (⋅) frs_tgt ε).
+  Let W: Type := (p_state).
+
+  Let r_state: Type := mname -> Σ.
+
+  Let zip_state (mps: p_state) (mrs: r_state): p_state :=
+    fun mn => match alist_find mn ms_tgt.(ModSemL.initial_mrs) with
+              | Some r => Any.pair (mps mn) (mrs mn)↑
+              | None => mps mn
+              end.
 
   Let rsum_minus (mn: mname): r_state -> Σ :=
-    fun '(mrs_tgt, frs_tgt) => (fold_left (⋅) (List.map ((update mrs_tgt mn ε) <*> fst) ms_tgt.(ModSemL.initial_mrs)) ε) ⋅ (fold_left (⋅) (tl frs_tgt) ε).
-
-
+    fun mrs_tgt => (fold_left (⋅) (List.map (mrs_tgt <*> fst) ms_tgt.(ModSemL.initial_mrs)) ε).
 
   Lemma fold_left_radd (r0 r1: Σ) rl
     :
@@ -198,13 +202,6 @@ Section CANCEL.
   Proof.
     revert r0 r1. induction rl; ss.
     i. rewrite <- URA.add_assoc. rewrite IHrl. auto.
-  Qed.
-
-  Lemma rsum_minus_spec mn mrs fhd ftl
-    :
-      rsum_minus mn (mrs, fhd::ftl) = rsum (update mrs mn ε, ftl).
-  Proof.
-    unfold rsum_minus, rsum. ss.
   Qed.
 
   Lemma fold_left_add (r: Σ) rs
@@ -216,77 +213,81 @@ Section CANCEL.
     i. rewrite IHrs. rewrite (IHrs (ε ⋅ a)). r_solve.
   Qed.
 
-  Lemma rsum_update mn mrs frs r
-        (NODUP: NoDup (List.map fst ms_tgt.(ModSemL.initial_mrs)))
-        (IN: List.In mn (List.map fst ms_tgt.(ModSemL.initial_mrs)))
-    :
-      rsum (update mrs mn r, frs) = rsum (update mrs mn ε, frs) ⋅ r.
-  Proof.
-    unfold rsum. rewrite <- URA.add_assoc. rewrite (URA.add_comm _ r).
-    rewrite URA.add_assoc. f_equal. unfold compose.
-    rewrite <- (List.map_map fst). rewrite <- (List.map_map fst). revert IN NODUP.
-    generalize (List.map fst (ModSemL.initial_mrs ms_tgt)) as mds0. i.
-    cut (forall r0 r1, fold_left URA.add (List.map (update mrs mn r0) mds0) ε ⋅ r1
-                       =
-                       fold_left URA.add (List.map (update mrs mn r1) mds0) ε ⋅ r0).
-    { i. specialize (H r ε). rewrite URA.unit_id in H. auto. }
-    i. revert mn r0 r1 IN NODUP. induction mds0; ss. i.
-    destruct (classic (In mn mds0)).
-    { clear IN. rewrite (fold_left_add (ε ⋅ update mrs mn r0 a)).
-      rewrite (fold_left_add (ε ⋅ update mrs mn r1 a)).
-      rewrite ! URA.unit_idl. rewrite <- URA.add_assoc. rewrite <- URA.add_assoc.
-      rewrite (URA.add_comm _ r1). rewrite (URA.add_comm _ r0).
-      rewrite URA.add_assoc. rewrite URA.add_assoc.
-      inv NODUP. rewrite IHmds0; ss.
-      f_equal. unfold update. des_ifs.
-    }
-    { des; ss. rewrite (fold_left_add (ε ⋅ update mrs mn r0 a)).
-      rewrite (fold_left_add (ε ⋅ update mrs mn r1 a)). subst.
-      unfold update at 2 4. des_ifs.
-      rewrite ! URA.unit_idl. rewrite <- URA.add_assoc. rewrite <- URA.add_assoc. f_equal.
-      { revert H. clear IHmds0 NODUP. induction mds0; ss. i.
-        rewrite (fold_left_add (ε ⋅ update mrs mn r0 a)).
-        rewrite (fold_left_add (ε ⋅ update mrs mn r1 a)).
-        rewrite IHmds0; auto. f_equal. f_equal.
-        unfold update. des_ifs; ss. exfalso. eapply H; auto.
-      }
-      { eapply URA.add_comm. }
-    }
-  Qed.
+  (* Lemma rsum_minus_spec mn mrs fhd ftl *)
+  (*   : *)
+  (*     rsum_minus mn (mrs, fhd::ftl) = rsum (update mrs mn ε, ftl). *)
+  (* Proof. *)
+  (*   unfold rsum_minus, rsum. ss. *)
+  (* Qed. *)
 
-  Lemma update_same A (mrs: string -> A) mn
-    :
-      update mrs mn (mrs mn) = mrs.
-  Proof.
-    extensionality mn0. unfold update. des_ifs.
-  Qed.
+  (* Lemma rsum_update mn mrs frs r *)
+  (*       (NODUP: NoDup (List.map fst ms_tgt.(ModSemL.initial_mrs))) *)
+  (*       (IN: List.In mn (List.map fst ms_tgt.(ModSemL.initial_mrs))) *)
+  (*   : *)
+  (*     rsum (update mrs mn r, frs) = rsum (update mrs mn ε, frs) ⋅ r. *)
+  (* Proof. *)
+  (*   unfold rsum. rewrite <- URA.add_assoc. rewrite (URA.add_comm _ r). *)
+  (*   rewrite URA.add_assoc. f_equal. unfold compose. *)
+  (*   rewrite <- (List.map_map fst). rewrite <- (List.map_map fst). revert IN NODUP. *)
+  (*   generalize (List.map fst (ModSemL.initial_mrs ms_tgt)) as mds0. i. *)
+  (*   cut (forall r0 r1, fold_left URA.add (List.map (update mrs mn r0) mds0) ε ⋅ r1 *)
+  (*                      = *)
+  (*                      fold_left URA.add (List.map (update mrs mn r1) mds0) ε ⋅ r0). *)
+  (*   { i. specialize (H r ε). rewrite URA.unit_id in H. auto. } *)
+  (*   i. revert mn r0 r1 IN NODUP. induction mds0; ss. i. *)
+  (*   destruct (classic (In mn mds0)). *)
+  (*   { clear IN. rewrite (fold_left_add (ε ⋅ update mrs mn r0 a)). *)
+  (*     rewrite (fold_left_add (ε ⋅ update mrs mn r1 a)). *)
+  (*     rewrite ! URA.unit_idl. rewrite <- URA.add_assoc. rewrite <- URA.add_assoc. *)
+  (*     rewrite (URA.add_comm _ r1). rewrite (URA.add_comm _ r0). *)
+  (*     rewrite URA.add_assoc. rewrite URA.add_assoc. *)
+  (*     inv NODUP. rewrite IHmds0; ss. *)
+  (*     f_equal. unfold update. des_ifs. *)
+  (*   } *)
+  (*   { des; ss. rewrite (fold_left_add (ε ⋅ update mrs mn r0 a)). *)
+  (*     rewrite (fold_left_add (ε ⋅ update mrs mn r1 a)). subst. *)
+  (*     unfold update at 2 4. des_ifs. *)
+  (*     rewrite ! URA.unit_idl. rewrite <- URA.add_assoc. rewrite <- URA.add_assoc. f_equal. *)
+  (*     { revert H. clear IHmds0 NODUP. induction mds0; ss. i. *)
+  (*       rewrite (fold_left_add (ε ⋅ update mrs mn r0 a)). *)
+  (*       rewrite (fold_left_add (ε ⋅ update mrs mn r1 a)). *)
+  (*       rewrite IHmds0; auto. f_equal. f_equal. *)
+  (*       unfold update. des_ifs; ss. exfalso. eapply H; auto. *)
+  (*     } *)
+  (*     { eapply URA.add_comm. } *)
+  (*   } *)
+  (* Qed. *)
 
-  Lemma rsum_cons mrs fhd ftl
-    :
-      rsum (mrs, fhd::ftl) = fhd ⋅ rsum (mrs, ftl).
-  Proof.
-    ss. transitivity (fold_left URA.add (List.map (mrs <*> fst) (ModSemL.initial_mrs ms_tgt)) ε
-                                ⋅ (fhd ⋅ fold_left URA.add ftl ε)).
-    { f_equal.
-      generalize fhd. generalize (@URA.unit (GRA.to_URA Σ)).
-      induction ftl; ss.
-      { i. r_solve. }
-      { i. ss.
-        replace (c ⋅ fhd0 ⋅ a) with ((c ⋅ a) ⋅ fhd0) by r_solve.
-        rewrite IHftl. r_solve.
-      }
-    }
-    { r_solve. }
-  Qed.
+  (* Lemma update_same A (mrs: string -> A) mn *)
+  (*   : *)
+  (*     update mrs mn (mrs mn) = mrs. *)
+  (* Proof. *)
+  (*   extensionality mn0. unfold update. des_ifs. *)
+  (* Qed. *)
 
-  Let wf: W -> W -> Prop :=
-    fun '((mrs_src, frs_src), mps_src) '((mrs_tgt, frs_tgt), mps_tgt) =>
-      (<<LEN: List.length frs_src = List.length frs_tgt>>) /\
-      (<<NNIL: frs_src <> [] >>) /\
-      (<<WFTGT: URA.wf (rsum (mrs_tgt, frs_tgt))>>) /\
-      (<<PHYS: mps_src = mps_tgt>>)
+  (* Lemma rsum_cons mrs fhd ftl *)
+  (*   : *)
+  (*     rsum (mrs, fhd::ftl) = fhd ⋅ rsum (mrs, ftl). *)
+  (* Proof. *)
+  (*   ss. transitivity (fold_left URA.add (List.map (mrs <*> fst) (ModSemL.initial_mrs ms_tgt)) ε *)
+  (*                               ⋅ (fhd ⋅ fold_left URA.add ftl ε)). *)
+  (*   { f_equal. *)
+  (*     generalize fhd. generalize (@URA.unit (GRA.to_URA Σ)). *)
+  (*     induction ftl; ss. *)
+  (*     { i. r_solve. } *)
+  (*     { i. ss. *)
+  (*       replace (c ⋅ fhd0 ⋅ a) with ((c ⋅ a) ⋅ fhd0) by r_solve. *)
+  (*       rewrite IHftl. r_solve. *)
+  (*     } *)
+  (*   } *)
+  (*   { r_solve. } *)
+  (* Qed. *)
+
+  Let wf: W -> W -> r_state -> Prop :=
+    fun mps_src mps_tgt mrs_tgt =>
+      mps_src = zip_state mps_tgt mrs_tgt
   .
-  Local Opaque rsum rsum_minus.
+  Local Opaque rsum_minus.
 
 
 
@@ -309,18 +310,61 @@ Section CANCEL.
   (*   forall [E : Type -> Type] [R U : Type] (e : E U) (k : U -> itree E R), ` x : U <- trigger e;; k x = Vis e (fun x : U => k x). *)
   (* Proof. i. eapply bind_trigger. Qed. *)
 
-  Let adequacy_type_aux:
+  Let zip_state_get st mrs mn
+      (MIN: List.In mn (List.map fst ms_tgt.(ModSemL.initial_mrs)))
+    :
+      zip_state st mrs mn = Any.pair (st mn) (mrs mn)↑.
+  Proof.
+    unfold zip_state. des_ifs.
+    eapply in_map_iff in MIN. des. destruct x. subst.
+    eapply alist_find_none in Heq.
+    exfalso. eapply Heq. et.
+  Qed.
+
+  Let zip_state_mput st mrs mn r
+      (MIN: List.In mn (List.map fst ms_tgt.(ModSemL.initial_mrs)))
+    :
+      update (zip_state st mrs) mn (Any.pair (st mn) (Any.upcast r))
+      =
+      zip_state st (update mrs mn r).
+  Proof.
+    extensionality mn0.
+    unfold update, zip_state. des_ifs.
+    eapply in_map_iff in MIN. des. destruct x. subst.
+    eapply alist_find_none in Heq.
+    exfalso. eapply Heq. et.
+  Qed.
+
+  (* Let zip_state_put st_tgt st_src mrs mn *)
+  (*     (ZIP: st_src = zip_state st_tgt mrs) *)
+  (*     (MIN: List.In mn (List.map fst ms_tgt.(ModSemL.initial_mrs))) *)
+  (*   : *)
+  (*     st_tgt mn = Any.pair (st_src mn) (mrs mn)↑. *)
+  (* Proof. *)
+  (*   admit "ez". *)
+  (* Qed. *)
+
+  Let adequacy_type_aux
+      (NODUP: NoDup (List.map fst ms_tgt.(ModSemL.initial_mrs))):
     forall RT
-           st_src0 st_tgt0 (SIM: wf st_src0 st_tgt0) (i0: itree (hCallE +' pE +' eventE) RT)
+           mrs0 frs fr0 ctx0
+           st_src0 st_tgt0 (i0: itree (hCallE +' pE +' eventE) RT)
            mn cur
-           rst (EQ: rst = fst st_tgt0)
+           (ZIP: st_tgt0 = zip_state st_src0 mrs0)
+           (CTX: ctx0 = frs ⋅ rsum_minus mn mrs0)
+           (RWF: URA.wf (fr0 ⋅ ctx0 ⋅ (mrs0 mn)))
+
            (MIN: List.In mn (List.map fst ms_tgt.(ModSemL.initial_mrs)))
            (NODUP: NoDup (List.map fst ms_tgt.(ModSemL.initial_mrs)))
     ,
-      simg (fun '((rs_src, v_src)) '((rs_tgt, v_tgt)) => wf rs_src rs_tgt /\ (v_src: RT) = snd v_tgt /\ (rsum_minus mn (fst rs_tgt)) = fst v_tgt)
+      simg (fun '(st_src1, v_src) '(st_tgt1, v_tgt) =>
+              exists mrs1 fr1,
+                (<<ZIP: st_tgt1 = zip_state st_src1 mrs1>>) /\
+                (<<RET: (v_tgt: Σ * Σ * RT) = (frs ⋅ rsum_minus mn mrs1, fr1, v_src)>>) /\
+                (<<RWF: URA.wf (fr1 ⋅ (frs ⋅ rsum_minus mn mrs1) ⋅ (mrs1 mn))>>))
            (Ord.from_nat 100%nat)
            (EventsL.interp_Es (ModSemL.prog ms_mid) (transl_all mn (interp_hCallE_mid (stb sk) cur i0)) st_src0)
-           (EventsL.interp_Es (ModSemL.prog ms_tgt) (transl_all mn (interp_hCallE_tgt mn (stb sk) cur i0 (rsum_minus mn rst))) st_tgt0)
+           (EventsL.interp_Es (ModSemL.prog ms_tgt) (transl_all mn (interp_hCallE_tgt mn (stb sk) cur i0 (ctx0, fr0))) st_tgt0)
   .
   Proof.
     Opaque subevent.
@@ -328,25 +372,30 @@ Section CANCEL.
     { i. eapply cpn6_wcompat; eauto with paco. }
     gcofix CIH. i; subst.
     ides i0; try rewrite ! unfold_interp; cbn; mred.
-    { steps. }
+    { steps. esplits; et. }
     { steps. gbase. eapply CIH; [..|M]; Mskip et. ss. }
-    destruct e; cycle 1.
+    rewrite <- bind_trigger. destruct e; cycle 1.
     {
       destruct s; ss.
       {
-        destruct st_src0 as [rst_src0 pst_src0], st_tgt0 as [rst_tgt0 pst_tgt0]; ss. des_ifs. des; clarify.
         destruct p; ss.
-        - rewrite <- bind_trigger. resub. steps. gbase. eapply CIH; ss.
-        - rewrite <- bind_trigger. resub. steps. gbase. eapply CIH; ss.
+        - resub. seal_left. steps. unfold pput. unseal_left. steps.
+          erewrite zip_state_get; et. rewrite Any.pair_split. steps.
+          gbase. eapply CIH; ss.
+          extensionality mn0. unfold update, zip_state. des_ifs.
+          exfalso. eapply in_map_iff in MIN. des. destruct x. subst.
+          eapply alist_find_none in Heq. et.
+        - resub. seal_left. steps. unfold pget. unseal_left. steps.
+          erewrite zip_state_get; et. rewrite Any.pair_split. steps.
+          gbase. eapply CIH; ss.
       }
       { dependent destruction e.
-        - rewrite <- bind_trigger. resub. steps. esplits; eauto. steps. gbase. eapply CIH; [..|M]; Mskip et. ss.
-        - rewrite <- bind_trigger. resub. steps. esplits; eauto. steps. gbase. eapply CIH; [..|M]; Mskip et. ss.
-        - rewrite <- bind_trigger. resub. steps. gbase. eapply CIH; [..|M]; Mskip et. ss.
+        - resub. steps. esplits; eauto. steps. gbase. eapply CIH; [..|M]; Mskip et. ss.
+        - resub. steps. esplits; eauto. steps. gbase. eapply CIH; [..|M]; Mskip et. ss.
+        - resub. steps. gbase. eapply CIH; [..|M]; Mskip et. ss.
       }
     }
-    dependent destruction h.
-    rewrite <- bind_trigger. resub.
+    dependent destruction h. resub.
     set (ModSemL.prog ms_mid) as p_mid in *.
     set (ModSemL.prog ms_tgt) as p_tgt in *.
     ss.
@@ -354,31 +403,27 @@ Section CANCEL.
 
     steps. hexploit (stb_find_iff fn). i. des.
     { rewrite NONE. steps. }
-    { rewrite FIND. unfold HoareCall, put, discard.
-      red in SIM. des_ifs. des. clarify. destruct l; ss.
-      steps. des. red in x5. uipropall. des; clarify.
-      ss. destruct tbr; ss.
-      { exfalso. hexploit TRIVIAL; et. i. subst. ss. hexploit x7; ss. }
+    { rewrite FIND. unfold HoareCall, mput, mget. steps.
+      erewrite zip_state_get; et. rewrite Any.pair_split. steps.
+      des; clarify. destruct tbr; ss.
+      { exfalso. hexploit TRIVIAL; et. i. subst. ss. hexploit x5; ss. }
       seal_right. unseal_left. steps. rewrite FIND. steps. esplits; et.
       steps. esplits; et.
-      { destruct cur; ss. hexploit x8; ss. i. subst. ss. }
+      { destruct cur; ss. hexploit x6; ss. i. subst. ss. }
       steps. rewrite FINDMID. steps.
     }
-    unfold HoareCall, put, guarantee, discard.
-
-    destruct st_tgt0 as [rst_tgt0 pst_tgt0]. destruct st_src0 as [rst_src0 pst_src0].
-    destruct rst_tgt0 as [mrs_tgt0 [|frs_tgt_hd frs_tgt_tl]] eqn:T; ss. steps.
-    { rr in SIM. des_ifs_safe. des; ss. destruct l; ss. }
+    unfold HoareCall, mput, mget.
 
     (*** exploiting both_tau ***)
     rewrite STB. ss. mred. force_r.
     destruct (classic (tbr = true /\ forall mn x arg_src arg_tgt o r (PRE: f.(precond) mn x arg_src arg_tgt o r), o = ord_top)).
-    { des. subst. steps. des. destruct f. ss. subst.
-      ss. red in x5. uipropall. des; subst. ss. exfalso.
-      hexploit H0; et. i. subst. ss. hexploit x7; ss.  }
+    { des. subst. steps.
+      erewrite zip_state_get; et. rewrite Any.pair_split. steps.
+      hexploit H0; et. i. subst. ss. des. hexploit x2; ss. }
     rename H into TRIVIAL.
     unseal_left. ired_both. rewrite STB. steps. esplit.
     { ii. subst. eapply TRIVIAL; ss. } steps.
+    erewrite zip_state_get; et. rewrite Any.pair_split. steps.
 
     match goal with
     | |- _ ?i_tgt => replace i_tgt with (Ret tt;;; i_tgt)
@@ -388,117 +433,71 @@ Section CANCEL.
     { instantiate (2:=(400+5)%ord).
       rewrite <- OrdArith.add_from_nat. refl. }
     guclo bindC_spec. econs.
-    { instantiate (1:= fun '(st_src, o) (_: unit) => st_src = (c, l, pst_src0) /\ o = x4).
+    { instantiate (1:= fun '(st_src, o) (_: unit) => st_src = st_src0 /\ o = x2).
       destruct tbr.
-      { steps. des. destruct x4; ss.
+      { steps. des. destruct x2; ss.
         { exists n. steps. }
-        { exfalso. hexploit x7; ss. }
+        { exfalso. hexploit x5; ss. }
       }
       { steps. des. splits; auto. symmetry. auto. }
     }
     i. destruct vret_src, vret_tgt. des; subst.
 
-    steps. esplits; eauto. steps. unshelve esplits; eauto. steps. unfold unwrapU.
+    steps. esplits; eauto. steps. unfold unwrapU.
     rewrite FINDMID. rewrite FINDTGT. rewrite ! bind_ret_l.
 
     guclo ordC_spec. econs.
-    { instantiate (1:=(192+200)%ord). rewrite <- OrdArith.add_from_nat. refl. }
+    { instantiate (1:=(195+200)%ord). rewrite <- OrdArith.add_from_nat. refl. }
     rename f into fs.
     guclo bindC_spec. econs.
 
-    { instantiate (1:= fun '(((mrs_src, frs_src), mps_src), vret_src)
-                           '(((mrs_tgt, frs_tgt), mps_tgt), vret_tgt) =>
-                         exists (rret: Σ),
-                           (<<ST: (List.length frs_src) = (List.length frs_tgt) /\
-                                  frs_src <> [] /\
-                                  URA.wf (rsum (mrs_tgt, rret :: frs_tgt))>>) /\
-                           (<<POST: fs.(postcond) (Some mn) x2 vret_src vret_tgt rret>>) /\
-                           (<<PHYS: mps_src = mps_tgt>>)
-                  ).
+    { instantiate (1:= fun '(st_src1, vret_src) '(st_tgt1, vret_tgt) =>
+                         exists (mrs1: r_state) rret,
+                           (<<ZIP: st_tgt1 = zip_state st_src1 mrs1>>) /\
+                           (<<POST: fs.(postcond) (Some mn) x0 vret_src vret_tgt rret>>) /\
+                           (<<RWF: URA.wf (rret ⋅ (c1 ⋅ (frs ⋅ rsum_minus mn mrs1) ⋅ (mrs1 mn)))>>)).
       fold sk. fold sk. set (mn0:=SModSem.mn (SMod.get_modsem md sk)) in *.
-      fold Any_tgt in x5.
-      unfold fun_to_src, fun_to_tgt, compose. des_ifs. unfold HoareFun.
-      rename x5 into PRECOND. rename x0 into rarg.
-      steps. exists (rsum_minus mn0 (update mrs_tgt0 mn c0, ε ⋅ rarg :: x1 :: frs_tgt_tl)).
+      fold Any_tgt in x3.
+      unfold fun_to_src, fun_to_tgt, compose. des_ifs. unfold HoareFun, mget, mput.
+      rename x3 into PRECOND. rename c0 into rarg.
+      steps. exists x0.
       steps. exists varg_src.
-      steps. esplits; et. steps. exists rarg.
-      steps. unfold forge, checkWf, assume, guarantee.
-      steps.
+      rewrite Any.pair_split. ired_both.
+      rewrite Any.upcast_downcast. ired_both. steps.
+      eexists (rarg, c1 ⋅ (frs ⋅ rsum_minus mn0 (update mrs0 mn c))).
+      steps. erewrite ! zip_state_mput; et.
+      erewrite zip_state_get; et.
+      rewrite Any.pair_split. steps. rewrite Any.upcast_downcast. steps.
       unshelve esplits; eauto.
-      { clear - rsum x MIN MIN0 NODUP.
-        rewrite rsum_minus_spec; auto. rewrite rsum_minus_spec in *; auto.
-        rewrite URA.add_assoc. rewrite <- rsum_update; auto.
-        erewrite update_same. rewrite rsum_update; auto.
-        rewrite rsum_cons.
-        replace (x1 ⋅ rsum (update mrs_tgt0 mn ε, frs_tgt_tl) ⋅ c0 ⋅ (ε ⋅ rarg))
-          with (rsum (update mrs_tgt0 mn ε, frs_tgt_tl) ⋅ (c0 ⋅ (rarg ⋅ x1))); auto.
-        r_solve.
-      }
+      { admit "ez". }
       steps. esplits; eauto. steps. unshelve esplits; eauto. steps.
-      unfold fun_to_mid.
-      rewrite Any.pair_split. ss. steps.
-      rewrite Any.upcast_downcast. steps.
       guclo ordC_spec. econs.
-      { instantiate (1:=(53+100)%ord). rewrite <- OrdArith.add_from_nat. refl. }
+      { instantiate (1:=(73+100)%ord). rewrite <- OrdArith.add_from_nat. refl. }
       guclo bindC_spec. econs.
-      { gbase. eapply CIH; ss. rr. esplits; ss; et. rewrite URA.unit_idl. clear - WFTGT x MIN MIN0 NODUP.
-        rewrite rsum_minus_spec in x; auto. rewrite URA.add_assoc in x.
-        rewrite <- rsum_update in x; auto.
-        rewrite rsum_cons. rewrite URA.add_comm.
-        rewrite rsum_cons. rewrite <- URA.add_assoc.
-        rewrite URA.add_comm. rewrite <- URA.add_assoc. auto. }
-      { ii. ss. des_ifs_safe. des; ss. clarify. destruct p, p0.
-        steps. esplits; eauto. steps. unfold put. steps. steps.
-        unfold handle_rE. destruct r0; ss. destruct l; ss.
-        { destruct r1. des; ss. }
-        steps.
-        unfold guarantee.
-        steps.
-        unfold discard.
-        steps. des. clarify. steps.
-        esplits; ss; eauto.
-        { rewrite rsum_minus_spec in x5; auto. rewrite URA.add_assoc in x5.
-          rewrite <- rsum_update in x5; auto.
-          rewrite rsum_cons. rewrite URA.add_comm.
-          rewrite rsum_cons. rewrite <- URA.add_assoc.
-          rewrite URA.add_comm. rewrite <- URA.add_assoc. auto.
-        }
+      { gbase. eapply CIH; ss.
+        { instantiate (1:=c1 ⋅ frs). r_solve. }
+        { admit "ez". }
+      }
+      { ii. ss. des_ifs_safe. des; ss. clarify.
+        steps. rewrite zip_state_get; et.
+        rewrite Any.pair_split. steps.
+        esplits; ss; et.
+        { admit "ez". }
       }
     }
-    { ii. ss. des_ifs_safe. des.
-      steps. esplits. steps.
-      unfold forge, checkWf, assume; steps.
-      des_ifs; ss.
-      { steps. }
-      steps. esplits. steps. instantiate (1:= rret).
-      exists (rsum_minus mn (c3, c6 ⋅ rret :: l1)). steps.
-      unshelve esplits; eauto.
-      { clear - ST1 MIN MIN0 NODUP. rewrite rsum_minus_spec; auto.
-        rewrite URA.add_assoc. rewrite <- rsum_update; auto.
-        rewrite update_same. eapply URA.wf_mon. instantiate (1:=c5).
-        rewrite ! rsum_cons in ST1.
-        replace (rsum (c3, l1) ⋅ (c6 ⋅ rret) ⋅ c5) with (rret ⋅ (c5 ⋅ (c6 ⋅ rsum (c3, l1)))); auto.
-        r_solve.
-      }
-      steps. unshelve esplits; eauto.
-      steps.
-      gbase. eapply CIH; ss.
-      rr. esplits; et. { destruct l2; ss. } clear - ST1.
-      eapply URA.wf_mon. instantiate (1:=c5).
-      rewrite ! rsum_cons. rewrite ! rsum_cons in ST1.
-      replace (c6 ⋅ rret ⋅ rsum (c3, l1) ⋅ c5) with (rret ⋅ (c5 ⋅ (c6 ⋅ rsum (c3, l1)))); auto.
-      r_solve.
+    { ii. ss. des_ifs_safe. des. subst.
+      steps. eexists (rret, frs ⋅ rsum_minus mn mrs1). steps.
+      rewrite zip_state_get; et.
+      rewrite Any.pair_split. steps. rewrite Any.upcast_downcast. steps.
+      unshelve esplits; et.
+      { admit "ez". }
+      steps. exists t. steps. unshelve esplits; et.
+      steps. gbase. eapply CIH; et.
+      { admit "ez". }
     }
   Unshelve.
-    all: try (by apply Ord.O).
-    all: try (by apply 0).
+    all: try (by exact 0).
   Qed.
-
-  Let initial_r_state ms entry_r: r_state :=
-    (fun mn => match alist_find mn ms.(ModSemL.initial_mrs) with
-               | Some r => fst r
-               | None => ε
-               end, [entry_r]). (*** we have a dummy-stack here ***)
 
   Opaque EventsL.interp_Es.
 
